src/arch/x64/X64.Semantics_s.fst
@@ -226,22 +226,22 @@ let eval_ins (ins:ins) : st unit =
   | IMul64 dst src ->
     check (valid_operand src);;
     update_operand dst ins (FStar.UInt.mul_mod #64 (eval_operand dst s) (eval_operand src s))
-    
+
   | Xor64 dst src ->
     check (valid_operand src);;
-    update_operand dst ins (FStar.UInt.logxor #64 (eval_operand dst s) (eval_operand src s))
+    update_operand dst ins (Types_s.logxor (eval_operand dst s) (eval_operand src s))
 
   | And64 dst src ->
     check (valid_operand src);;
-    update_operand dst ins (FStar.UInt.logand #64 (eval_operand dst s) (eval_operand src s))
+    update_operand dst ins (Types_s.logand (eval_operand dst s) (eval_operand src s))
 
   | Shr64 dst amt ->
     check (valid_shift_operand amt);;
-    update_operand dst ins (FStar.UInt.shift_right #64 (eval_operand dst s) (eval_operand amt s))
+    update_operand dst ins (Types_s.shift_right (eval_operand dst s) (eval_operand amt s))
 
   | Shl64 dst amt ->
     check (valid_shift_operand amt);;
-    update_operand dst ins (FStar.UInt.shift_left #64 (eval_operand dst s) (eval_operand amt s))
+    update_operand dst ins (Types_s.shift_left (eval_operand dst s) (eval_operand amt s))
 
 (*
  * these functions return an option state
