src/crypto/poly1305/Poly1305.Spec_s.fst
@@ -1,17 +1,13 @@
 module Poly1305.Spec_s
 
 open FStar.Mul
-open FStar.UInt
-
-let nat128_max = 0x100000000000000000000000000000000
-let _ = assert_norm (pow2 128 = nat128_max) 
-type nat128 = x:int{0 <= x && x < nat128_max}
+open Types_s
 
 let modp'(x:int):int =
   x % (nat128_max * 4 - 5)
 
-let and128 (x:nat128) (y:nat128) :nat128 =
-  logand #128 x y
+let and128 (x:nat128) (y:nat128) : nat128 =
+  logand x y
 
 let rec poly1305_hash_blocks (h:int) (pad:int) (r:int) (inp:int->nat128) (k:nat) : Tot int =
   if k = 0 then h
@@ -21,7 +17,7 @@ let rec poly1305_hash_blocks (h:int) (pad:int) (r:int) (inp:int->nat128) (k:nat)
     modp' ((hh + pad + inp kk) * r)
 
 let poly1305_hash (key_r:nat128) (key_s:nat128) (inp:int->nat128) (len:nat) :int =
-  let r = logand #128 key_r 0x0ffffffc0ffffffc0ffffffc0fffffff in
+  let r = logand key_r 0x0ffffffc0ffffffc0ffffffc0fffffff in
   let nBlocks = len / 16 in
   let nExtra = len % 16 in
   let padBlocks = nat128_max in
